backend/ConventionsC.v
@@ -5,39 +5,4 @@ Require Export Conventions1.
 (* newly added *)
 Require Export Conventions.
 
-Local Opaque Z.add Z.mul Z.divide list_nth_z.
-Lemma tailcall_size_aux
-      tys ir fr
-      (TAIL: forall l,
-          In l (regs_of_rpairs (loc_arguments_64 tys ir fr 0)) ->
-          match l with
-          | R _ => True
-          | S _ _ _ => False
-          end)
-      (IRBOUND: (ir - 1) < list_length_z int_param_regs)
-      (FRBOUND: (fr - 1) < list_length_z float_param_regs)
-  :
-    <<SZ: size_arguments_64 tys ir fr 0 = 0>>
-.
-Proof.
-  ginduction tys; ii; ss.
-  destruct a; des_ifs; ss;
-    try (by exploit TAIL; eauto; ss);
-    (eapply IHtys; eauto;
-     [ii; des_ifs; []; exploit TAIL; eauto
-     |rewrite Z.add_simpl_r; apply list_nth_z_range in Heq; xomega]).
-Qed.
-
-Lemma tailcall_size
-      sg
-      (TAIL: tailcall_possible sg)
-  :
-    size_arguments sg = 0
-.
-Proof.
-  eapply tailcall_size_aux; eauto; cbn; xomega.
-Qed.
-
-Definition agree_callee_save_regs (ls1 ls2: Locmap.t) : Prop :=
-  forall r, is_callee_save r -> ls1 (R r) = ls2 (R r).
-
+Global Instance main_args_some: main_args_ctx := { main_args := true }.
